\documentclass[a4paper,10pt,american]{article}
\usepackage[left=2cm,right=2cm,top=2cm,bottom=2cm]{geometry}
\usepackage{amsmath}
\begin{document}

\title{Assignment 2}
\author{Yunhao Huang}
\date{\today}

\maketitle

\newcommand\foc[1]{\frac{\partial\mathcal{L}}{\partial{#1}}}


\begin{enumerate}
	\item 
	\begin{enumerate}
		\item 
		Construct the household's consumption Lagrangian function:
		\begin{align*}
		\mathcal{L}=\sum_{t=0}^{\infty} \beta^t \left( \frac{C_t^{1-\sigma}}{1-\sigma}-\frac{H_t^{1+\psi}}{1+\psi}\right) +\sum_{t=0}^{\infty} \lambda_t \left[ {\omega_t(1-\tau_t^\omega)H_t+(1+r_{t-1})A_t+T_t-C_t-A_{t+1}} \right]
		\end{align*}
		The first-order conditions are
		\begin{align*}
			C_t &: \quad \beta^t C_t^{-\sigma} -\lambda_t=0 \\
			A_{t+1} &: \quad \lambda_{t+1}(1+r_t)-\lambda_t=0\\
			H_t &: \quad -\beta^t H_t^\psi +\lambda_t\omega_t(1-\tau_t^\omega)=0\\
			\lambda_t &: \quad \omega_t(1-\tau_t^\omega)H_t+(1+r_{t-1})A_t+T_t-C_t-A_{t+1}=0
		\end{align*}
		Using the FOCs of $C_t$ and $A_{t+1}$, we get the Euler equation
		\begin{align*}
		C_t^{-\sigma}=\beta (1+r_t) C_{t+1}^{-\sigma} \iff C_t=\beta ^\sigma (1+r_t)^\sigma C_{t+1}
		\end{align*}
		Using the FOCs of $H_t$ and $C_t$, we get the optimal condition for labor supply
		\begin{align*}
		\frac{H_t^\psi}{C_t^{-\sigma}}=\omega_t(1-\tau_t^\omega)
		\end{align*}
		
		\item
		Construct the firm's profit Lagrangian function:
		\begin{align*}
		\mathcal{L}=\sum_{t=0}^{\infty} (Y_t-\omega_t H_t) +\sum_{t=0}^{\infty} \lambda_t(Y_t-H_t)
		\end{align*}
		The first-order conditions are:
		\begin{align*}
		H_t &: \quad \lambda_t+\omega_t=0\\
		\lambda_t &: \quad Y_t-H_t=0
		\end{align*}
	\end{enumerate}

	
	\item
	\begin{enumerate}
		\item 
		
	\end{enumerate}
	
	
	
\end{enumerate}

\end{document}